{
 "cells": [
  {
   "cell_type": "markdown",
   "metadata": {},
   "source": [
    "# 1"
   ]
  },
  {
   "cell_type": "markdown",
   "metadata": {},
   "source": [
    "### 1(a)"
   ]
  },
  {
   "cell_type": "markdown",
   "metadata": {},
   "source": [
    "Note that\n",
    "\n",
    "$$\\begin{align*}\n",
    "b^Tx=\n",
    "\\begin{bmatrix}b_1&\\dots&b_n\\end{bmatrix}\\begin{bmatrix}x_1\\\\\\vdots\\\\x_n\\end{bmatrix}=\\sum_{i=1}^nb_ix_i\\end{align*}$$\n",
    "\n",
    "Hence\n",
    "\n",
    "$$\\begin{align*}\n",
    "\\frac{\\partial b^Tx}{\\partial x_i}=b_i\\end{align*}$$\n",
    "\n",
    "And\n",
    "\n",
    "$$\\nabla_x (b^Tx)=\\begin{bmatrix}\\frac{\\partial b^Tx}{\\partial x_1}\\\\\\vdots\\\\\\frac{\\partial b^Tx}{\\partial x_n}\\end{bmatrix}=\\begin{bmatrix}b_1\\\\\\vdots\\\\b_n\\end{bmatrix} = b$$"
   ]
  },
  {
   "cell_type": "markdown",
   "metadata": {},
   "source": [
    "Similarly for $x^TAx$:\n",
    "\n",
    "$$\\begin{align*}\n",
    "x^TAx &= x^T(Ax) \\\\\n",
    "&= x^T\n",
    "\\begin{bmatrix}\n",
    " A_1 x \\\\ \n",
    " A_2 x \\\\\n",
    " \\cdots \\\\\n",
    " A_n x\n",
    "\\end{bmatrix} \\\\\n",
    "&= \\begin{bmatrix}x_{1}&\\dots&x_{n}\\end{bmatrix}\n",
    "\\begin{bmatrix}\n",
    " \\sum_{j=1}^{n} A_{1j} x_j \\\\ \n",
    " \\sum_{j=1}^{n} A_{2j} x_j \\\\\n",
    " \\cdots \\\\\n",
    " \\sum_{j=1}^{n} A_{nj} x_j\n",
    "\\end{bmatrix} \\\\\n",
    "&= x_1\\sum_{j=1}^{n} A_{1j} x_j + x_2\\sum_{j=1}^{n} A_{2j} x_j + \\cdots + x_n \\sum_{j=1}^{n} A_{nj} x_j \\\\\n",
    "&= \\sum_{i=1}^n \\sum_{j=1}^{n} x_i A_{ij} x_j \\\\\n",
    "&= \\sum_{i=1}^n \\sum_{j=1}^{n} A_{ij} x_i x_j\n",
    "\\end{align*}$$\n",
    "\n",
    "Next, in the second equality, we split out the double sum into the three disjoint cases: (1) neither $i$ nor $j$ equals $k$, (2) exactly one of $i$ or $j$ equals $k$, and (3) both equal $k$:\n",
    "\n",
    "$$\\begin{align*}\n",
    "\\frac{\\partial x^TAx}{\\partial x_k}&=\\frac{\\partial \\sum_{j=1}^n \\sum_{i=1}^{n} A_{ij} x_i x_j}{\\partial x_k}\\\\\n",
    "&=\\frac{\\partial \\big(\\sum_{j=1,j\\neq k}^n \\sum_{i=1,i\\neq k}^{n} A_{ij} x_i x_j+\\sum_{i=k}^k\\sum_{j=1,j\\neq k}^{n} A_{ij} x_i x_j+\\sum_{j=k}^k\\sum_{i=1,i\\neq k}^{n} A_{ij} x_i x_j+A_{kk}x_kx_k\\big)}{\\partial x_k}\\\\\n",
    "&=\\frac{\\partial \\big(\\sum_{j=1,j\\neq k}^n \\sum_{i=1,i\\neq k}^{n} A_{ij} x_i x_j+\\sum_{j=1,j\\neq k}^{n} A_{kj} x_k x_j+\\sum_{i=1,i\\neq k}^{n} A_{ik} x_i x_k+A_{kk}x_k^2\\big)}{\\partial x_k}\\\\\n",
    "&=\\frac{\\partial \\big(\\sum_{j=1,j\\neq k}^{n} A_{kj} x_k x_j+\\sum_{i=1,i\\neq k}^{n} A_{ik} x_i x_k+A_{kk}x_k^2\\big)}{\\partial x_k}\\\\\n",
    "&=\\frac{\\partial \\big(\\sum_{j=1,j\\neq k}^{n} A_{kj} x_k x_j+\\sum_{i=1,i\\neq k}^{n} A_{ki} x_k x_i+A_{kk}x_k^2\\big)}{\\partial x_k}\\tag{A symmetric}\\\\\n",
    "&=\\frac{\\partial \\big(2\\sum_{j=1,j\\neq k}^{n} A_{kj} x_k x_j+A_{kk}x_k^2\\big)}{\\partial x_k}\\\\\n",
    "&=\\frac{\\partial \\big(2\\sum_{j=1,j\\neq k}^{n} A_{kj} x_k x_j\\big)}{\\partial x_k}+\\frac{\\partial A_{kk}x_k^2}{\\partial x_k}\\\\\n",
    "&=2\\sum_{j=1,j\\neq k}^{n}\\frac{\\partial A_{kj} x_k x_j}{\\partial x_k}+2A_{kk}x_k\\\\\n",
    "&= 2 \\sum_{j = 1,j\\neq k}^{n} A_{kj}x_j+2A_{kk}x_k \\\\\n",
    "&= 2 \\sum_{j = 1}^{n} A_{kj}x_j \\\\\n",
    "&= 2 \\begin{bmatrix}A_{k1}&\\dots&A_{kn}\\end{bmatrix}\\begin{bmatrix}x_1\\\\\\vdots\\\\x_n\\end{bmatrix} \\\\\n",
    "&= 2 A_k x \\\\\n",
    "\\end{align*}$$\n",
    "\n",
    "Hence the gradient is\n",
    "\n",
    "$$\\begin{align*}\n",
    "\\nabla_x (x^TAx) = \\begin{bmatrix}\\frac{\\partial x^T(Ax)}{\\partial x_1}\\\\\\vdots\\\\\\frac{\\partial x^T(Ax)}{\\partial x_n}\\end{bmatrix}\n",
    "= 2 \\begin{bmatrix}A_1 x\\\\\\vdots\\\\A_n x\n",
    "\\end{bmatrix} = 2Ax\n",
    "\\end{align*}$$\n",
    "\n",
    "And the answer to the question is\n",
    "\n",
    "$$\\nabla_x f(x) = \\nabla_x \\Big(\\frac{1}{2} x^T A x + b^T x\\Big) = \\frac{1}{2}\\nabla_xx^TAx + \\nabla_xb^Tx = Ax + b$$,\n",
    "\n",
    "which is analogous to the univariate case:\n",
    "\n",
    "$$\\frac{d(\\frac{1}{2}ax^2 + bx)}{dx} = ax + b$$."
   ]
  },
  {
   "cell_type": "markdown",
   "metadata": {},
   "source": [
    "### 1(b)"
   ]
  },
  {
   "cell_type": "markdown",
   "metadata": {},
   "source": [
    "The chain rule gives\n",
    "\n",
    "$$\\begin{align*}\n",
    "\\frac{\\partial f(x)}{\\partial x_i}=\\frac{\\partial g(h(x))}{\\partial x_i}=g'(h(x))\\frac{\\partial h(x)}{\\partial x_i}\n",
    "\\end{align*}$$\n",
    "\n",
    "Hence\n",
    "\n",
    "$$\\begin{align*}\n",
    "\\nabla_xf(x) = \\begin{bmatrix}\\frac{\\partial f(x)}{\\partial x_1}\\\\\\vdots\\\\\\frac{\\partial f(x)}{\\partial x_n}\\end{bmatrix}= \\begin{bmatrix}g'(h(x))\\frac{\\partial h(x)}{\\partial x_1}\\\\\\vdots\\\\g'(h(x)) \\frac{\\partial h(x)}{\\partial x_n} \\\\\\end{bmatrix}=g'(h(x))\\begin{bmatrix}\\frac{\\partial h(x)}{\\partial x_1}\\\\\\vdots\\\\ \\frac{\\partial h(x)}{\\partial x_n} \\\\\\end{bmatrix}=g'(h(x))\\nabla_xh(x)\n",
    "\\end{align*}$$"
   ]
  },
  {
   "cell_type": "markdown",
   "metadata": {},
   "source": [
    "### 1(c)"
   ]
  },
  {
   "cell_type": "markdown",
   "metadata": {},
   "source": [
    "Part (a) gives\n",
    "\n",
    "$$\n",
    "\\frac{\\partial^2 b^Tx}{\\partial x_k \\partial x_l}=\\frac{\\partial b_l}{\\partial x_k}=0\n",
    "$$\n",
    "\n",
    "So the Hessian is\n",
    "\n",
    "$$\n",
    "\\nabla_x^2b^Tx=\\begin{bmatrix}\\frac{\\partial^2 b^Tx}{\\partial x_1 \\partial x_1}&\\dots&\\frac{\\partial^2 b^Tx}{\\partial x_1 \\partial x_n}\\\\\\vdots&\\ddots&\\vdots\\\\\\frac{\\partial^2 b^Tx}{\\partial x_n \\partial x_1}&\\dots&\\frac{\\partial^2 b^Tx}{\\partial x_n \\partial x_n}\\end{bmatrix}=\\begin{bmatrix}0&\\dots&0\\\\\\vdots&\\ddots&\\vdots\\\\0&\\dots&0\\end{bmatrix}=0\n",
    "$$\n",
    "\n",
    "Part (a) gives\n",
    "\n",
    "$$\\begin{align*}\n",
    "\\frac{\\partial x^TAx}{\\partial x_k}=2A_k x=2 \\begin{bmatrix}A_{k1}&\\dots&A_{kn}\\end{bmatrix}\\begin{bmatrix}x_1\\\\\\vdots\\\\x_n\\end{bmatrix}\n",
    "=2\\sum_{j = 1}^{n} A_{kj}x_j \\\\\n",
    "\\end{align*}$$\n",
    "\n",
    "Hence $x^TAx$ is twice continuously differentible and\n",
    "\n",
    "$$\\begin{align*}\n",
    "\\frac{\\partial^2 x^TAx}{\\partial x_k\\partial x_l}=\\frac{\\partial^2 x^TAx}{\\partial x_l\\partial x_k}=2\\frac{\\partial\\sum_{j = 1}^{n} A_{kj}x_j}{\\partial x_l}=2A_{kl} \\\\\n",
    "\\end{align*}$$\n",
    "\n",
    "So the Hessian is\n",
    "\n",
    "$$\n",
    "\\nabla_x^2x^TAx=\\begin{bmatrix}\\frac{\\partial^2 x^TAx}{\\partial x_1 \\partial x_1}&\\dots&\\frac{\\partial^2 x^TAx}{\\partial x_1 \\partial x_n}\\\\\\vdots&\\ddots&\\vdots\\\\\\frac{\\partial^2 x^TAx}{\\partial x_n \\partial x_1}&\\dots&\\frac{\\partial^2 x^TAx}{\\partial x_n \\partial x_n}\\end{bmatrix}=\\begin{bmatrix}2A_{11}&\\dots&2A_{1n}\\\\\\vdots&\\ddots&\\vdots\\\\2A_{n1}&\\dots&2A_{nn}\\end{bmatrix}=2\\begin{bmatrix}A_{11}&\\dots&A_{1n}\\\\\\vdots&\\ddots&\\vdots\\\\A_{n1}&\\dots&A_{nn}\\end{bmatrix}=2A\n",
    "$$\n",
    "\n",
    "and the solution is\n",
    "\n",
    "$$\n",
    "\\nabla_x^2 f(x) = \\nabla_x^2 \\Big(\\frac{1}{2}x^T A x + b^Tx\\Big)=\\frac{1}{2}2A=A\n",
    "$$\n",
    "\n",
    "which is analogous to\n",
    "\n",
    "$$\\frac{d^2(\\frac{1}{2}ax^2 + bx)}{dx^2} = a$$.\n",
    "\n",
    "__Corrolary:__ $w(x)=x^Tx$ is convex.\n",
    "\n",
    "__Proof__ Recall that $w$ is convex if and only if its Hessian is positive semi-definite. Note that\n",
    "\n",
    "$$\n",
    "\\nabla_x^2w(x)=\\nabla_x^2x^TIx=2I\n",
    "$$\n",
    "\n",
    "and for any vector $v\\in\\mathbb{R}^n$\n",
    "\n",
    "$$\n",
    "v^T2Iv=2v^Tv=2\\lvert v\\rvert^2=2\\sum_iv_i^2>0\n",
    "$$\n",
    "\n",
    "$\\blacksquare$\n",
    "\n",
    "__Corrolary:__ Affine functions are convex.\n",
    "\n",
    "__Proof__ For $a\\in\\mathbb{R}$, let $q(x)=b^Tx+a$. Note that\n",
    "\n",
    "$$\n",
    "\\nabla_x^2q(x)=\\nabla_x^2(b^Tx)+\\nabla_x^2(a)=0_{n\\times n}\n",
    "$$\n",
    "\n",
    "and for any vector $v\\in\\mathbb{R}^n$\n",
    "\n",
    "$$\n",
    "v^T0v=0\n",
    "$$\n",
    "\n",
    "$\\blacksquare$"
   ]
  },
  {
   "cell_type": "markdown",
   "metadata": {},
   "source": [
    "### 1(d)"
   ]
  },
  {
   "cell_type": "markdown",
   "metadata": {},
   "source": [
    "Define $h(x)=a^Tx$ so that $h:\\mathbb{R}^n\\mapsto\\mathbb{R}$ and $f(x)=g\\circ h(x)$. Then part (a) gives $\\nabla_xh(x)=a$ and part (b) gives\n",
    "\n",
    "$$\\nabla_xf(x)=g'(h(x))\\nabla_xh(x) = g'(a^Tx) \\cdot a$$\n",
    "\n",
    "Part (b) also gives the partials:\n",
    "\n",
    "$$\\begin{align*}\n",
    "\\frac{\\partial g\\circ h(x)}{\\partial x_i}=g'(h(x))\\frac{\\partial h(x)}{\\partial x_i}=g'(a^Tx)a_i\n",
    "\\end{align*}$$\n",
    "\n",
    "Since $f=g\\circ h$ is twice continuously differentiable, then the second partials are\n",
    "\n",
    "$$\\begin{align*}\n",
    "\\frac{\\partial^2 f(x)}{\\partial x_i\\partial x_j}=\\frac{\\partial^2 g\\circ h(x)}{\\partial x_j\\partial x_i}=\\frac{\\partial g'(a^Tx)a_i}{\\partial x_j}=a_i\\frac{\\partial g'(\\sum_{k=1}^na_kx_k)}{\\partial x_j}=a_ia_jg''(a^Tx)\n",
    "\\end{align*}$$\n",
    "\n",
    "And the Hessian is\n",
    "\n",
    "$$\\begin{align*}\n",
    "\\nabla_x^2f(x)=\\begin{bmatrix}a_1a_1g''(a^Tx)&\\dots&a_1a_ng''(a^Tx)\\\\\\vdots&\\ddots&\\vdots\\\\a_na_1g''(a^Tx)&\\dots&a_na_ng''(a^Tx)\\end{bmatrix}=g''(a^Tx)\\begin{bmatrix}a_1a_1&\\dots&a_1a_n\\\\\\vdots&\\ddots&\\vdots\\\\a_na_1&\\dots&a_na_n\\end{bmatrix}=g''(a^Tx)\\begin{bmatrix}a_1\\\\\\dots\\\\a_n\\end{bmatrix}\\begin{bmatrix}a_1&\\dots&a_n\\end{bmatrix}=g''(a^Tx)aa^T\n",
    "\\end{align*}$$"
   ]
  },
  {
   "cell_type": "markdown",
   "metadata": {},
   "source": [
    "# 2"
   ]
  },
  {
   "cell_type": "markdown",
   "metadata": {},
   "source": [
    "### 2(a)\n",
    "\n",
    "Part 1.\n",
    "\n",
    "Given $A = zz^T$, so $A^T = z^T z = A$. Besides, $A_{ij} = z_i z_j$.\n",
    "\n",
    "\n",
    "Part 2. Following 1(a)\n",
    "\n",
    "\\begin{align*}\n",
    "x^T A x &= \\sum_{i=1}^n \\sum_{j=1}^{n} A_{ij} x_i x_j \\\\\n",
    "        &= \\sum_{i=1}^n \\sum_{j=1}^{n} z_i z_j x_i x_j \\\\\n",
    "        &= \\sum_{i=1}^n \\sum_{j=1}^{n} (z_i x_i) (z_j x_j) \\\\\n",
    "        &= (\\sum_{i=1}^{n} z_i x_i)^2 \\\\\n",
    "        &\\ge = 0\n",
    "\\end{align*}\n",
    "\n",
    "Because $A = A^T$ and $x^T A x \\ge 0$, so A is positive semidefinite (PSD)."
   ]
  },
  {
   "cell_type": "markdown",
   "metadata": {},
   "source": [
    "### 2(b)\n",
    "\n",
    "\\begin{align*}\n",
    "A &= zz^T \\\\\n",
    "  &= \n",
    "\\begin{bmatrix}\n",
    " z_1 z_1 & z_1 z_2 & \\cdots & z_1 z_n \\\\ \n",
    " z_2 z_1 & z_2 z_2 & \\cdots & z_2 z_n \\\\\n",
    " \\cdots & \\cdots & \\ddots & \\cdots \\\\\n",
    " z_n z_1 & z_n z_2 & \\cdots & z_n z_n\n",
    "\\end{bmatrix} \\\\\n",
    "& \\rightarrow \n",
    "\\begin{bmatrix}\n",
    " z_1 z_1 & z_1 z_2 & \\cdots & z_1 z_n \\\\ \n",
    " 0 & 0 & \\cdots & 0 \\\\\n",
    " \\cdots & \\cdots & \\ddots & \\cdots \\\\\n",
    " 0 & 0 & \\cdots & 0\n",
    "\\end{bmatrix} \\\\\n",
    " &= z_1\n",
    "\\begin{bmatrix}\n",
    " z_1 & z_2 & \\cdots & z_n \\\\ \n",
    " 0 & 0 & \\cdots & 0 \\\\\n",
    " \\cdots & \\cdots & \\ddots & \\cdots \\\\\n",
    " 0 & 0 & \\cdots & 0\n",
    "\\end{bmatrix} \\\\\n",
    " &= R \\\\\n",
    "\\end{align*}\n",
    "\n",
    "The $\\rightarrow$ means row transformation by multiplying row $1$ with $-\\frac{z_i}{z_1}$, and add it to row $i$. This is possible because $z$ is given as a _non-zero n-vector_.\n",
    "\n",
    "So the rank of $A$ is $1$.\n",
    "\n",
    "To obtain its nullspace, we need to find all possible $x$ vectors that satisfy $Ax = 0$, Before that, let's consider the dimensions of four fundamental subspaces in linear algebra:\n",
    "\n",
    "\n",
    "|                | Symbol   | Dimension | Note                                                                                |\n",
    "|----------------|----------|-----------|-------------------------------------------------------------------------------------|\n",
    "| Row space      | $C(A^T)$ | 1         | Equal to rank                                                                                    |\n",
    "| Column space   | $C(A)$   | 1         | Equal to rank                                                                       |\n",
    "| Nullspace      | $N(A)$   | n - 1     | Usually the dimension of nullspace is $m - 1$, but given A is symmetric, so $m = n$ |\n",
    "| Left nullspace | $N(A^T)$ | n - 1     | - |\n",
    "\n",
    "Therefore, the nullspace of $A$ consists of $n-1$ vectors, which could be derived from $n-1$ free variables. Result:\n",
    "\n",
    "\\begin{align*}\n",
    "Ax &= 0 \\\\\n",
    "Rx &= 0 \\\\\n",
    "z_1 \\sum_{i=1}^{n} z_i x_i & = 0 \\\\\n",
    "\\sum_{i=1}^{n} z_i x_i &= 0\n",
    "\\end{align*}"
   ]
  },
  {
   "cell_type": "markdown",
   "metadata": {},
   "source": [
    "Therefore, by setting any of the $n=1$ free variables to $1$, and the rest to $0$, and then calculating a value for the pivot variable ($x_1$), we can obtain $n-1$ independent vectors for $x$, and by multiplying each vector with an arbitrary constant, we obtain the nullspace, i.e. all possible vectors that satisfy $Ax = 0$.\n",
    "\n",
    "\\begin{align*}\n",
    "N(A) &=\n",
    "c_2 \\begin{bmatrix}\n",
    " -z_2/z_1 \\\\ \n",
    " 1 \\\\\n",
    " 0 \\\\\n",
    " 0 \\\\\n",
    " \\vdots \\\\\n",
    " 0\n",
    "\\end{bmatrix} + \n",
    "c_3 \\begin{bmatrix}\n",
    " -z_3/z_1 \\\\\n",
    " 0 \\\\\n",
    " 1 \\\\\n",
    " 0 \\\\\n",
    " \\vdots \\\\\n",
    " 0\n",
    "\\end{bmatrix} +\n",
    "\\cdots +\n",
    "c_i \\begin{bmatrix}\n",
    " -z_i/z_1 \\\\\n",
    " 0 \\\\\n",
    " \\vdots \\\\\n",
    " 1 \\\\\n",
    " \\vdots \\\\\n",
    " 0\n",
    "\\end{bmatrix} + \n",
    "\\cdots +\n",
    "c_n \\begin{bmatrix}\n",
    " -z_n/z_1 \\\\\n",
    " 0 \\\\\n",
    " 0 \\\\\n",
    " 0 \\\\\n",
    " \\vdots \\\\\n",
    " 1\n",
    "\\end{bmatrix} \\\\\n",
    "&= \\sum_{k=2}^n c_k \\begin{bmatrix}\n",
    " -z_k/z_1 \\\\\n",
    " I\\{i=k\\} \\\\\n",
    " I\\{i=k\\} \\\\\n",
    " \\vdots \\\\\n",
    " I\\{i=k\\}\n",
    "\\end{bmatrix}\n",
    "\\end{align*}\n",
    "\n",
    "where $i$ is the row index, $I$ is an indicator function, and $c_k$ is a constant. Note, $k$ starts from $2$ instead of $1$. This is meaningful only when $z_1$ is non-zero."
   ]
  },
  {
   "cell_type": "markdown",
   "metadata": {},
   "source": [
    "### 2(c)"
   ]
  },
  {
   "cell_type": "markdown",
   "metadata": {},
   "source": [
    "Given \n",
    "\n",
    "1. $A \\in \\mathbb{R}^{n\\times n}$ is PSD, so $A = A^T$, and $x^T A x \\ge 0$, and \n",
    "1. $B \\in \\mathbb{R}^{m\\times n}$\n",
    "\n",
    "Let's denote $C = BAB^T$. We need to prove two parts in order to show that $C$ is PSD, too.\n",
    "\n",
    "Part 1.\n",
    "\n",
    "\\begin{align*}\n",
    "C^T &= (BAB^T)^T \\\\\n",
    "    &= (B^T)^T A^T B^T \\\\\n",
    "    &= B A^T B^T \\\\\n",
    "    &= B A B^T \\\\\n",
    "    &= C\n",
    "\\end{align*}\n",
    "\n",
    "Part 2.\n",
    "\\begin{align*}\n",
    "x^T C x &= x^T (BAB^T) x \\\\\n",
    "        &= (x^T B) A (B^T x) \\\\\n",
    "        &= (B^T x)^T A (B^T x) \\\\\n",
    "        &= y^T A y \\\\\n",
    "        &\\ge 0\n",
    "\\end{align*}\n",
    "\n",
    "Here we transformed $x^T C x$ into one that leverages the property of A, $x^T A x \\ge 0$, by setting $y = B^T x$. Therefore, $BAB^T$ is PSD.\n"
   ]
  },
  {
   "cell_type": "markdown",
   "metadata": {},
   "source": [
    "# 3"
   ]
  },
  {
   "cell_type": "markdown",
   "metadata": {},
   "source": [
    "### 3(a)\n",
    "\n",
    "Given $A = T \\Lambda T^{-1}$, so\n",
    "\n",
    "\\begin{align*}\n",
    "            & A T = T \\Lambda \\\\\n",
    "\\rightarrow & A[t^{(1)} \\cdots t^{(n)}] = [t^{(1)} \\cdots t^{(n)}] \\Lambda \\\\\n",
    "\\rightarrow & At^{(i)} = t^{(i)} \\lambda_i \\\\\n",
    "\\end{align*}\n",
    "\n",
    "The last step is because $\\Lambda$ is a diagonal matrix with all off-diagonal values being zeros. Therefore, \n",
    "\n",
    "$$ At^{(i)} = \\lambda_i t^{(i)} $$\n",
    "\n",
    "$(t^{(i)}, \\lambda_i)$ is an eigenvalue/eigenvector pair."
   ]
  },
  {
   "cell_type": "markdown",
   "metadata": {},
   "source": [
    "### 3(b)\n",
    "\n",
    "##### **Spectral theorem (important!)**: \n",
    "\n",
    "If $A \\in \\mathbb{R}^{n \\times n}$ is **symetric** (i.e. $A = A^T$), then $A$ is **diagonalizable** ($\\Lambda$) by a **real** **orthogonal** ($U$) matrix. In symbols, \n",
    "\n",
    "$$ U^T A U = \\Lambda$$\n",
    "\n",
    "or equivalently,\n",
    "\n",
    "$$ A = U \\Lambda U^T$$\n"
   ]
  },
  {
   "cell_type": "markdown",
   "metadata": {},
   "source": [
    "Given $A = A^T$, and $U$ is orthogonal, and $A = U \\Lambda U^T$, then\n",
    "\n",
    "$$AU = U \\Lambda U^T U = U \\Lambda$$\n",
    "\n",
    "Following the same logic as in **3(a)**, we get\n",
    "\n",
    "$$Au^{(i)} = \\lambda_i u^{(i)}$$\n",
    "\n",
    "so $u^{(i)}$ is an eigenvector."
   ]
  },
  {
   "cell_type": "markdown",
   "metadata": {},
   "source": [
    "### 3(c)\n",
    "\n",
    "Given $A$ is PSD, so\n",
    "\n",
    "\\begin{align*}\n",
    "x^T A x &= x^TU \\Lambda U^T x \\\\\n",
    "        &= (U^Tx)^T \\Lambda (U^Tx) \\\\\n",
    "        &= y^T \\Lambda y \\\\\n",
    "        &= \\sum_{i} y_i^2 \\lambda_i \\\\\n",
    "        &\\ge 0\n",
    "\\end{align*}\n",
    "\n",
    "The last inequality uses the property of a PSD matrix. Here $y$ = $U^Tx$. Since $y_i^2 \\ge 0 $, and $x$ is arbitray, to guarantee $x^T A x \\ge 0$ for all $x$s, then all $\\lambda_i$ should be $\\ge 0$. (Please let me know if there is a better way to show this)"
   ]
  },
  {
   "cell_type": "code",
   "execution_count": null,
   "metadata": {
    "collapsed": true
   },
   "outputs": [],
   "source": []
  }
 ],
 "metadata": {
  "anaconda-cloud": {},
  "kernelspec": {
   "display_name": "Python 3",
   "language": "python",
   "name": "python3"
  },
  "language_info": {
   "codemirror_mode": {
    "name": "ipython",
    "version": 3
   },
   "file_extension": ".py",
   "mimetype": "text/x-python",
   "name": "python",
   "nbconvert_exporter": "python",
   "pygments_lexer": "ipython3",
   "version": "3.6.1"
  }
 },
 "nbformat": 4,
 "nbformat_minor": 2
}
