{
 "cells": [
  {
   "cell_type": "markdown",
   "metadata": {},
   "source": [
    "## Ex.1\n",
    "\n",
    "Define $f(x)\\equiv c_1x_1+c_2x_2$. Then\n",
    "\n",
    "$$\\begin{align*} \n",
    "\\frac{\\partial f(x)}{\\partial x_i}=\\frac{\\partial(c_1x_1+c_2x_2)}{\\partial x_i}=c_i\n",
    "\\end{align*}$$\n",
    "\n",
    "Let $A$ be a 2x2 matrix. Define g(x)=f(Ax). Then\n",
    "\n",
    "$$\\begin{align*} \n",
    "g(x)=f(Ax) &= f\\Bigg(\\begin{bmatrix}a_{11}&a_{12}\\\\a_{21}&a_{22}\\end{bmatrix}\\begin{bmatrix}x_1\\\\x_2\\end{bmatrix}\\Bigg) \\\\\n",
    "    &= f\\Bigg(\\begin{bmatrix}a_{11}x_1+a_{12}x_2\\\\a_{21}x_1+a_{22}x_2\\end{bmatrix}\\Bigg) \\\\\n",
    "    &= f\\Bigg(\\begin{bmatrix}(Ax)_1\\\\(Ax)_2\\end{bmatrix}\\Bigg) \\\\\n",
    "    &= c_1(Ax)_1+c_2(Ax)_2 \\\\\n",
    "    &= c_1(a_{11}x_1+a_{12}x_2)+c_2(a_{21}x_1+a_{22}x_2)\n",
    "\\end{align*}$$\n",
    "\n",
    "Hence\n",
    "\n",
    "$$\\begin{align*} \n",
    "\\frac{\\partial g(x)}{\\partial x_1}=c_1a_{11}+c_2a_{21}\n",
    "\\end{align*}$$\n",
    "\n",
    "or we can notice that $Ax$ is a vector-valued function of $x_1$ and use the [chain rule](https://www.khanacademy.org/math/multivariable-calculus/multivariable-derivatives/differentiating-vector-valued-functions/a/multivariable-chain-rule-simple-version):\n",
    "\n",
    "$$\\begin{align*} \n",
    "\\frac{\\partial g(x)}{\\partial x_1} &= \\nabla_{(Ax)}f(Ax)\\cdot\\frac{\\partial (Ax)}{\\partial x_1} \\\\\n",
    "    &= \\begin{bmatrix}\\frac{\\partial f(Ax)}{\\partial (Ax)_1}\\\\ \\frac{\\partial f(Ax)}{\\partial (Ax)_2}\\end{bmatrix}\\cdot\\begin{bmatrix}\\frac{\\partial(Ax)_1}{\\partial x_1}\\\\\\frac{\\partial(Ax)_2}{\\partial x_1}\\end{bmatrix} \\\\\n",
    "    &= \\sum_{k=1}^2\\frac{\\partial f(Ax)}{\\partial(Ax)_k}\\frac{\\partial(Ax)_k}{\\partial x_1} \\\\\n",
    "    &= \\frac{\\partial f(Ax)}{\\partial(Ax)_1}\\frac{\\partial(Ax)_1}{\\partial x_1}+\\frac{\\partial f(Ax)}{\\partial(Ax)_2}\\frac{\\partial(Ax)_2}{\\partial x_1} \\\\\n",
    "    &= \\frac{\\partial[c_1(Ax)_1+c_2(Ax)_2]}{\\partial(Ax)_1}\\frac{\\partial[a_{11}x_1+a_{12}x_2]}{\\partial x_1}+\\frac{\\partial [c_1(Ax)_1+c_2(Ax)_2]}{\\partial(Ax)_2}\\frac{\\partial[a_{21}x_1+a_{22}x_2]}{\\partial x_1} \\\\\n",
    "    &= c_1a_{11}+c_2a_{21}\n",
    "\\end{align*}$$"
   ]
  },
  {
   "cell_type": "markdown",
   "metadata": {},
   "source": [
    "## Ex.2\n",
    "\n",
    "Define $f(x)\\equiv x_1x_2$. Then\n",
    "\n",
    "$$\n",
    "\\begin{align*} \n",
    "\\frac{\\partial f(x)}{\\partial x_1}=\\frac{\\partial(x_1x_2)}{\\partial x_i}=x_2\n",
    "\\end{align*}\n",
    "$$\n",
    "\n",
    "Let $A$ be a 2x2 matrix. Define g(x)=f(Ax). Then\n",
    "\n",
    "$$\n",
    "\\begin{align*} \n",
    "g(x)=f(Ax) &= f\\Bigg(\\begin{bmatrix}a_{11}&a_{12}\\\\a_{21}&a_{22}\\end{bmatrix}\\begin{bmatrix}x_1\\\\x_2\\end{bmatrix}\\Bigg) \\\\\n",
    "    &= f\\Bigg(\\begin{bmatrix}a_{11}x_1+a_{12}x_2\\\\a_{21}x_1+a_{22}x_2\\end{bmatrix}\\Bigg) \\\\\n",
    "    &= f\\Bigg(\\begin{bmatrix}(Ax)_1\\\\(Ax)_2\\end{bmatrix}\\Bigg) \\\\\n",
    "    &= (Ax)_1(Ax)_2 \\\\\n",
    "    &= (a_{11}x_1+a_{12}x_2)(a_{21}x_1+a_{22}x_2) \\\\\n",
    "    &= a_{11}x_1a_{21}x_1+a_{11}x_1a_{22}x_2+a_{12}x_2a_{21}x_1+a_{12}x_2a_{22}x_2 \\\\\n",
    "    &= a_{11}a_{21}x_1^2+a_{11}x_1a_{22}x_2+a_{12}x_2a_{21}x_1+a_{12}a_{22}x_2^2\n",
    "\\end{align*}\n",
    "$$\n",
    "\n",
    "Hence\n",
    "\n",
    "$$\n",
    "\\begin{align*} \n",
    "\\frac{\\partial g(x)}{\\partial x_1}=2a_{11}a_{21}x_1+a_{11}a_{22}x_2+a_{12}x_2a_{21}\n",
    "\\end{align*}\n",
    "$$\n",
    "\n",
    "or we can notice that $Ax$ is a vector-valued function of $x_1$ and use the [chain rule](https://www.khanacademy.org/math/multivariable-calculus/multivariable-derivatives/differentiating-vector-valued-functions/a/multivariable-chain-rule-simple-version):\n",
    "\n",
    "$$\n",
    "\\begin{align*} \n",
    "\\frac{\\partial g(x)}{\\partial x_1} &= \\nabla_{(Ax)}f(Ax)\\cdot\\frac{\\partial (Ax)}{\\partial x_1} \\\\\n",
    "    &= \\begin{bmatrix}\\frac{\\partial f(Ax)}{\\partial (Ax)_1}\\\\ \\frac{\\partial f(Ax)}{\\partial (Ax)_2}\\end{bmatrix}\\cdot\\begin{bmatrix}\\frac{\\partial(Ax)_1}{\\partial x_1}\\\\\\frac{\\partial(Ax)_2}{\\partial x_1}\\end{bmatrix} \\\\\n",
    "    &= \\sum_{k=1}^2\\frac{\\partial f(Ax)}{\\partial(Ax)_k}\\frac{\\partial(Ax)_k}{\\partial x_1} \\\\\n",
    "    &= \\frac{\\partial f(Ax)}{\\partial(Ax)_1}\\frac{\\partial(Ax)_1}{\\partial x_1}+\\frac{\\partial f(Ax)}{\\partial(Ax)_2}\\frac{\\partial(Ax)_2}{\\partial x_1} \\\\\n",
    "    &= \\frac{\\partial[(Ax)_1(Ax)_2]}{\\partial(Ax)_1}\\frac{\\partial[a_{11}x_1+a_{12}x_2]}{\\partial x_1}+\\frac{\\partial [(Ax)_1(Ax)_2]}{\\partial(Ax)_2}\\frac{\\partial[a_{21}x_1+a_{22}x_2]}{\\partial x_1} \\\\\n",
    "    &= (Ax)_2a_{11}+(Ax)_1a_{21} \\\\\n",
    "    &= (a_{21}x_1+a_{22}x_2)a_{11}+(a_{11}x_1+a_{12}x_2)a_{21} \\\\\n",
    "    &= a_{11}a_{21}x_1+a_{11}a_{22}x_2+a_{11}a_{21}x_1+a_{12}a_{21}x_2 \\\\\n",
    "    &= 2a_{11}a_{21}x_1+a_{11}a_{22}x_2+a_{12}a_{21}x_2\n",
    "\\end{align*}\n",
    "$$\n",
    "\n",
    "To compute the Jacobian, define $h(x)=Ax$ so that $g(x)=(f\\circ h)(x)$. Note that $g:\\mathbb{R}^2\\mapsto\\mathbb{R}$ so its Jacobian is $Dg(x)\\in\\mathbb{R}^{1\\times2}$.\n",
    "\n",
    "$$\n",
    "\\begin{align*} \n",
    "Dh(x)=J_xh(x)=A\n",
    "\\end{align*}\n",
    "$$\n",
    "\n",
    "$$\n",
    "\\begin{align*} \n",
    "Df(x)=J_xf(x)=\\begin{bmatrix}\\frac{\\partial f_1}{\\partial x_1}&\\frac{\\partial f_1}{\\partial x_2}\\end{bmatrix}=\\begin{bmatrix}x_2&x_1\\end{bmatrix}\n",
    "\\end{align*}\n",
    "$$\n",
    "\n",
    "$$\n",
    "\\begin{align*} \n",
    "Dg(x)=J_xg(x)&=Df(h(x))\\circ Dh(x)=Df(Ax)\\circ A=\\begin{bmatrix}(Ax)_2&(Ax)_1\\end{bmatrix}\\begin{bmatrix}a_{11}&a_{12}\\\\a_{21}&a_{22}\\end{bmatrix}=\\begin{bmatrix}a_{21}x_1+a_{22}x_2&a_{11}x_1+a_{12}x_2\\end{bmatrix}\\begin{bmatrix}a_{11}&a_{12}\\\\a_{21}&a_{22}\\end{bmatrix}\\\\\n",
    "    &=\\begin{bmatrix}(a_{21}x_1+a_{22}x_2)a_{11}+(a_{11}x_1+a_{12}x_2)a_{21}&(a_{21}x_1+a_{22}x_2)a_{12}+(a_{11}x_1+a_{12}x_2)a_{22}\\end{bmatrix}\\\\\n",
    "    &=\\begin{bmatrix}a_{11}a_{21}x_1+a_{11}a_{22}x_2+a_{21}a_{11}x_1+a_{21}a_{12}x_2&a_{12}a_{21}x_1+a_{12}a_{22}x_2+a_{22}a_{11}x_1+a_{22}a_{12}x_2\\end{bmatrix}\\\\\n",
    "    &=\\begin{bmatrix}2a_{11}a_{21}x_1+a_{11}a_{22}x_2+a_{12}a_{21}x_2&a_{12}a_{21}x_1+2a_{12}a_{22}x_2+a_{11}a_{22}x_1\\end{bmatrix}\n",
    "\\end{align*}\n",
    "$$\n",
    "\n",
    "Let's compute the partial derivative using Jacobians. Fix $x_2\\in\\mathbb{R}$ and define $w:\\mathbb{R}\\mapsto\\mathbb{R}^2$ as\n",
    "\n",
    "$$w(x_1)\\equiv\\begin{bmatrix}x_1\\\\x_2\\end{bmatrix}$$\n",
    "\n",
    "Then\n",
    "\n",
    "$$Dw(x_1)=J_w(x_1)=\\begin{bmatrix}1\\\\0\\end{bmatrix}$$\n",
    "\n",
    "Then $g(x_1)=(f\\circ h\\circ w)(x_1)$ so $Dg(x_1)=D(f\\circ h\\circ w)(x_1)$ and \n",
    "\n",
    "$$\n",
    "\\begin{align*}\n",
    "Dg(x_1)&=D(f\\circ h\\circ w)(x_1)=Df(h(w(x_1)))\\circ Dh(w(x_1))\\circ Dw(x_1)\\\\\n",
    "    &=Df\\Big(A\\begin{bmatrix}x_1\\\\x_2\\end{bmatrix}\\Big)\\circ Dh\\Big(\\begin{bmatrix}x_1\\\\x_2\\end{bmatrix}\\Big)\\circ\\begin{bmatrix}1\\\\0\\end{bmatrix}\\\\\n",
    "    &=Df\\Big(\\begin{bmatrix}a_{11}&a_{12}\\\\a_{21}&a_{22}\\end{bmatrix}\\begin{bmatrix}x_1\\\\x_2\\end{bmatrix}\\Big)\\circ A\\begin{bmatrix}1\\\\0\\end{bmatrix}\\\\\n",
    "    &=Df\\Big(\\begin{bmatrix}a_{11}x_1+a_{12}x_2\\\\a_{21}x_1+a_{22}x_2\\end{bmatrix}\\Big)\\circ \\begin{bmatrix}a_{11}&a_{12}\\\\a_{21}&a_{22}\\end{bmatrix}\\begin{bmatrix}1\\\\0\\end{bmatrix}\\\\\n",
    "    &=\\begin{bmatrix}a_{21}x_1+a_{22}x_2&a_{11}x_1+a_{12}x_2\\end{bmatrix} \\begin{bmatrix}a_{11}&a_{12}\\\\a_{21}&a_{22}\\end{bmatrix}\\begin{bmatrix}1\\\\0\\end{bmatrix}\\\\\n",
    "    &=\\begin{bmatrix}a_{21}x_1+a_{22}x_2&a_{11}x_1+a_{12}x_2\\end{bmatrix} \\begin{bmatrix}a_{11}\\\\a_{21}\\end{bmatrix} \\\\\n",
    "    &= (a_{21}x_1+a_{22}x_2)a_{11}+(a_{11}x_1+a_{12}x_2)a_{21} \\\\\n",
    "    &= a_{11}a_{21}x_1+a_{11}a_{22}x_2+a_{11}a_{21}x_1+a_{12}a_{21}x_2 \\\\\n",
    "    &= 2a_{11}a_{21}x_1+a_{11}a_{22}x_2+a_{12}a_{21}x_2\n",
    "\\end{align*}\n",
    "$$"
   ]
  },
  {
   "cell_type": "markdown",
   "metadata": {
    "collapsed": true
   },
   "source": [
    "## Ex.3\n",
    "\n",
    "Define $f:\\mathbb{R}^2\\mapsto\\mathbb{R}$ and $g:\\mathbb{R}\\mapsto\\mathbb{R}$ as\n",
    "\n",
    "$$\n",
    "\\begin{align*} \n",
    "g(y)\\equiv By=b_{11}y\n",
    "\\quad\\quad\n",
    "f(x)\\equiv Ax=\\begin{bmatrix}a_{11}&a_{12}\\end{bmatrix}\\begin{bmatrix}x_{1}\\\\x_{2}\\end{bmatrix}\n",
    "\\end{align*}\n",
    "$$\n",
    "\n",
    "Then the composite $g\\circ f:\\mathbb{R}^2\\mapsto\\mathbb{R}$ is\n",
    "\n",
    "$$\n",
    "\\begin{align*} \n",
    "(g\\circ f)(x)=g\\big(f(x)\\big)=b_{11}\\begin{bmatrix}a_{11}&a_{12}\\end{bmatrix}\\begin{bmatrix}x_{1}\\\\x_{2}\\end{bmatrix}\n",
    "=b_{11}(a_{11}x_1+a_{12}x_2)=b_{11}a_{11}x_1+b_{11}a_{12}x_2\n",
    "\\end{align*}\n",
    "$$\n",
    "\n",
    "A cursery derivative is\n",
    "\n",
    "$$\n",
    "\\begin{align*} \n",
    "D(g\\circ f)(x)=J_x(g\\circ f)(x)=\\begin{bmatrix}\\frac{\\partial (g\\circ f)}{\\partial x_1}&\\frac{\\partial (g\\circ f)}{\\partial x_2}\\end{bmatrix}=\\begin{bmatrix}b_{11}a_{11}&b_{11}a_{12}\\end{bmatrix}=b_{11}\\begin{bmatrix}a_{11}&a_{12}\\end{bmatrix}\n",
    "\\end{align*}\n",
    "$$\n",
    "\n",
    "Or we can look at each derivative\n",
    "\n",
    "$$\n",
    "\\begin{align*} \n",
    "Dg(y)=b_{11}=B\\quad\\quad Df(x)=J_xf(x)=\\begin{bmatrix}a_{11}&a_{12}\\end{bmatrix}=A\n",
    "\\end{align*}\n",
    "$$\n",
    "\n",
    "And use the chain rule\n",
    "\n",
    "$$\n",
    "\\begin{align*} \n",
    "D(g\\circ f)(x)=Dg(f(x))\\circ Df(x)=b_{11}\\begin{bmatrix}a_{11}&a_{12}\\end{bmatrix}=BA\n",
    "\\end{align*}\n",
    "$$"
   ]
  },
  {
   "cell_type": "markdown",
   "metadata": {
    "collapsed": true
   },
   "source": [
    "## Ex.4\n",
    "\n",
    "Define $f:\\mathbb{R}^2\\mapsto\\mathbb{R}^2$ and $g:\\mathbb{R}^2\\mapsto\\mathbb{R}$ as\n",
    "\n",
    "$$\n",
    "\\begin{align*} \n",
    "g(y)\\equiv By=\\begin{bmatrix}b_{11}&b_{12}\\end{bmatrix}\\begin{bmatrix}y_1\\\\y_2\\end{bmatrix}=b_{11}y_1+b_{12}y_2\n",
    "\\end{align*}\n",
    "$$\n",
    "\n",
    "$$\n",
    "\\begin{align*} \n",
    "f(x)\\equiv Ax=\\begin{bmatrix}a_{11}&a_{12}\\\\a_{21}&a_{22}\\end{bmatrix}\\begin{bmatrix}x_{1}\\\\x_{2}\\end{bmatrix}=\\begin{bmatrix}a_{11}x_{1}+a_{12}x_{2}\\\\a_{21}x_{1}+a_{22}x_{2}\\end{bmatrix}\n",
    "\\end{align*}\n",
    "$$\n",
    "\n",
    "Then the composite $g\\circ f:\\mathbb{R}^2\\mapsto\\mathbb{R}$ is\n",
    "\n",
    "$$\n",
    "\\begin{align*} \n",
    "(g\\circ f)(x)&=g\\big(f(x)\\big)=g\\Bigg(\\begin{bmatrix}a_{11}x_{1}+a_{12}x_{2}\\\\a_{21}x_{1}+a_{22}x_{2}\\end{bmatrix}\n",
    "\\Bigg)=\\begin{bmatrix}b_{11}&b_{12}\\end{bmatrix}\\begin{bmatrix}a_{11}x_{1}+a_{12}x_{2}\\\\a_{21}x_{1}+a_{22}x_{2}\\end{bmatrix}\\\\\n",
    "    &=b_{11}(a_{11}x_{1}+a_{12}x_{2})+b_{12}(a_{21}x_{1}+a_{22}x_{2})=b_{11}a_{11}x_{1}+b_{11}a_{12}x_{2}+b_{12}a_{21}x_{1}+b_{12}a_{22}x_{2}\\\\\n",
    "    &=(b_{11}a_{11}+b_{12}a_{21})x_1+(b_{11}a_{12}+b_{12}a_{22})x_2\n",
    "\\end{align*}\n",
    "$$\n",
    "\n",
    "A cursery derivative is\n",
    "\n",
    "$$\n",
    "\\begin{align*} \n",
    "D(g\\circ f)(x)=J_x(g\\circ f)(x)=\\begin{bmatrix}\\frac{\\partial (g\\circ f)}{\\partial x_1}&\\frac{\\partial (g\\circ f)}{\\partial x_2}\\end{bmatrix}=\\begin{bmatrix}b_{11}a_{11}+b_{12}a_{21}&b_{11}a_{12}+b_{12}a_{22}\\end{bmatrix}\n",
    "\\end{align*}\n",
    "$$\n",
    "\n",
    "Or we can look at each derivative\n",
    "\n",
    "$$\n",
    "\\begin{align*} \n",
    "Dg(y)=J_yg(y)=\\begin{bmatrix}\\frac{\\partial g}{\\partial y_1}&\\frac{\\partial g}{\\partial y_2}\\end{bmatrix}=\\begin{bmatrix}b_{11}&b_{12}\\end{bmatrix}=B\n",
    "\\end{align*}\n",
    "$$\n",
    "\n",
    "$$\n",
    "\\begin{align*} \n",
    "Df(x)=J_xf(x)=\\begin{bmatrix}\\frac{\\partial f_1}{\\partial x_1}&\\frac{\\partial f_1}{\\partial x_2}\\\\\\frac{\\partial f_2}{\\partial x_1}&\\frac{\\partial f_2}{\\partial x_2}\\end{bmatrix}=\\begin{bmatrix}a_{11}&a_{12}\\\\a_{21}&a_{22}\\end{bmatrix}\n",
    "\\end{align*}=A\n",
    "$$\n",
    "\n",
    "And use the chain rule\n",
    "\n",
    "$$\n",
    "\\begin{align*} \n",
    "D(g\\circ f)(x)=Dg(f(x))\\circ Df(x)=\\begin{bmatrix}b_{11}&b_{12}\\end{bmatrix}\\begin{bmatrix}a_{11}&a_{12}\\\\a_{21}&a_{22}\\end{bmatrix}=\\begin{bmatrix}b_{11}a_{11}+b_{12}a_{21}&b_{11}a_{12}+b_{12}a_{22}\\end{bmatrix}=BA\n",
    "\\end{align*}\n",
    "$$"
   ]
  },
  {
   "cell_type": "markdown",
   "metadata": {
    "collapsed": true
   },
   "source": [
    "## Ex.5\n",
    "\n",
    "Define $f:\\mathbb{R}^2\\mapsto\\mathbb{R}^2$ and $g:\\mathbb{R}^2\\mapsto\\mathbb{R}^2$ as\n",
    "\n",
    "$$\n",
    "\\begin{align*} \n",
    "g(y)\\equiv By=\\begin{bmatrix}b_{11}&b_{12}\\\\b_{21}&b_{22}\\end{bmatrix}\\begin{bmatrix}y_1\\\\y_2\\end{bmatrix}=\\begin{bmatrix}b_{11}y_1+b_{12}y_2\\\\b_{21}y_1+b_{22}y_2\\end{bmatrix}\n",
    "\\end{align*}\n",
    "$$\n",
    "\n",
    "$$\n",
    "\\begin{align*} \n",
    "f(x)\\equiv Ax=\\begin{bmatrix}a_{11}&a_{12}\\\\a_{21}&a_{22}\\end{bmatrix}\\begin{bmatrix}x_{1}\\\\x_{2}\\end{bmatrix}=\\begin{bmatrix}a_{11}x_{1}+a_{12}x_{2}\\\\a_{21}x_{1}+a_{22}x_{2}\\end{bmatrix}\n",
    "\\end{align*}\n",
    "$$\n",
    "\n",
    "Then the composite $g\\circ f:\\mathbb{R}^2\\mapsto\\mathbb{R}^2$ is\n",
    "\n",
    "$$\n",
    "\\begin{align*} \n",
    "(g\\circ f)(x)&=g\\big(f(x)\\big)=g\\Bigg(\\begin{bmatrix}a_{11}x_{1}+a_{12}x_{2}\\\\a_{21}x_{1}+a_{22}x_{2}\\end{bmatrix}\n",
    "\\Bigg)=\\begin{bmatrix}b_{11}&b_{12}\\\\b_{21}&b_{22}\\end{bmatrix}\\begin{bmatrix}a_{11}x_{1}+a_{12}x_{2}\\\\a_{21}x_{1}+a_{22}x_{2}\\end{bmatrix}\\\\\n",
    "    &=\\begin{bmatrix}b_{11}(a_{11}x_{1}+a_{12}x_{2})+b_{12}(a_{21}x_{1}+a_{22}x_{2})\\\\b_{21}(a_{11}x_{1}+a_{12}x_{2})+b_{22}(a_{21}x_{1}+a_{22}x_{2})\\end{bmatrix}\\\\\n",
    "    &=\\begin{bmatrix}b_{11}a_{11}x_{1}+b_{11}a_{12}x_{2}+b_{12}a_{21}x_{1}+b_{12}a_{22}x_{2}\\\\b_{21}a_{11}x_{1}+b_{21}a_{12}x_{2}+b_{22}a_{21}x_{1}+b_{22}a_{22}x_{2}\\end{bmatrix}\\\\\n",
    "    &=\\begin{bmatrix}(b_{11}a_{11}+b_{12}a_{21})x_1+(b_{11}a_{12}+b_{12}a_{22})x_2\\\\(b_{21}a_{11}+b_{22}a_{21})x_1+(b_{21}a_{12}+b_{22}a_{22})x_2\\end{bmatrix}\n",
    "\\end{align*}\n",
    "$$\n",
    "\n",
    "A cursery derivative is\n",
    "\n",
    "$$\n",
    "\\begin{align*} \n",
    "D(g\\circ f)(x)=J_x(g\\circ f)(x)=\\begin{bmatrix}\\frac{\\partial (g\\circ f)_1}{\\partial x_1}&\\frac{\\partial (g\\circ f)_1}{\\partial x_2}\\\\\\frac{\\partial (g\\circ f)_2}{\\partial x_1}&\\frac{\\partial (g\\circ f)_2}{\\partial x_2}\\end{bmatrix}=\\begin{bmatrix}b_{11}a_{11}+b_{12}a_{21}&b_{11}a_{12}+b_{12}a_{22}\\\\b_{21}a_{11}+b_{22}a_{21}&b_{21}a_{12}+b_{22}a_{22}\\end{bmatrix}\n",
    "\\end{align*}\n",
    "$$\n",
    "\n",
    "Or we can look at each derivative\n",
    "\n",
    "$$\n",
    "\\begin{align*} \n",
    "Dg(y)=J_yg(y)=\\begin{bmatrix}\\frac{\\partial g_1}{\\partial y_1}&\\frac{\\partial g_1}{\\partial y_2}\\\\\\frac{\\partial g_2}{\\partial y_1}&\\frac{\\partial g_2}{\\partial y_2}\\end{bmatrix}=\\begin{bmatrix}b_{11}&b_{12}\\\\b_{21}&b_{22}\\end{bmatrix}=B\n",
    "\\end{align*}\n",
    "$$\n",
    "\n",
    "$$\n",
    "\\begin{align*} \n",
    "Df(x)=J_xf(x)=\\begin{bmatrix}\\frac{\\partial f_1}{\\partial x_1}&\\frac{\\partial f_1}{\\partial x_2}\\\\\\frac{\\partial f_2}{\\partial x_1}&\\frac{\\partial f_2}{\\partial x_2}\\end{bmatrix}=\\begin{bmatrix}a_{11}&a_{12}\\\\a_{21}&a_{22}\\end{bmatrix}=A\n",
    "\\end{align*}\n",
    "$$\n",
    "\n",
    "And use the chain rule\n",
    "\n",
    "$$\n",
    "\\begin{align*} \n",
    "D(g\\circ f)(x)=Dg(f(x))\\circ Df(x)=\\begin{bmatrix}b_{11}&b_{12}\\\\b_{21}&b_{22}\\end{bmatrix}\\begin{bmatrix}a_{11}&a_{12}\\\\a_{21}&a_{22}\\end{bmatrix}=\\begin{bmatrix}b_{11}a_{11}+b_{12}a_{21}&b_{11}a_{12}+b_{12}a_{22}\\\\b_{21}a_{11}+b_{22}a_{21}&b_{21}a_{12}+b_{22}a_{22}\\end{bmatrix}=BA\n",
    "\\end{align*}\n",
    "$$"
   ]
  },
  {
   "cell_type": "code",
   "execution_count": null,
   "metadata": {
    "collapsed": true
   },
   "outputs": [],
   "source": []
  }
 ],
 "metadata": {
  "kernelspec": {
   "display_name": "Python 3",
   "language": "python",
   "name": "python3"
  },
  "language_info": {
   "codemirror_mode": {
    "name": "ipython",
    "version": 3
   },
   "file_extension": ".py",
   "mimetype": "text/x-python",
   "name": "python",
   "nbconvert_exporter": "python",
   "pygments_lexer": "ipython3",
   "version": "3.6.1"
  }
 },
 "nbformat": 4,
 "nbformat_minor": 2
}
